coq/cclc/clc_typing.v
@@ -7,44 +7,44 @@ Set Implicit Arguments.
 Unset Strict Implicit.
 Unset Printing Implicit Defensive.
 
-Reserved Notation "Γ |- m : A " (at level 50, m, A at next level).
+Reserved Notation "Γ ⊢ m : A" (at level 50, m, A at next level).
 
 Inductive clc_type : context term -> term -> term -> Prop :=
 | clc_axiom Γ s l :
   Γ |> U ->
-  Γ |- s @ l : U @ l.+1
+  Γ ⊢ s @ l : U @ l.+1
 | clc_pi Γ A B s r t i :
   Γ |> U ->
-  Γ |- A : s @ i ->
-  [A :{s} Γ] |- B : r @ i ->
-  Γ |- Pi A B s t : t @ i
+  Γ ⊢ A : s @ i ->
+  [A :{s} Γ] ⊢ B : r @ i ->
+  Γ ⊢ Pi A B s t : t @ i
 | clc_var Γ x A s :
   has Γ x s A ->
-  Γ |- Var x : A
+  Γ ⊢ Var x : A
 | clc_lam Γ A B m s r t i :
   Γ |> t ->
-  [Γ] |- Pi A B s t : r @ i ->
-  A :{s} Γ |- m : B ->
-  Γ |- Lam A m s t : Pi A B s t
+  [Γ] ⊢ Pi A B s t : r @ i ->
+  A :{s} Γ ⊢ m : B ->
+  Γ ⊢ Lam A m s t : Pi A B s t
 | clc_app Γ1 Γ2 Γ A B m n s t :
   Γ2 |> s ->
   Γ1 + Γ2 => Γ ->
-  Γ1 |- m : Pi A B s t ->
-  Γ2 |- n : A ->
-  Γ |- App m n : B.[n/]
+  Γ1 ⊢ m : Pi A B s t ->
+  Γ2 ⊢ n : A ->
+  Γ ⊢ App m n : B.[n/]
 | clc_conv Γ A B m s i :
   A <: B ->
-  Γ |- m : A ->
-  [Γ] |- B : s @ i ->
-  Γ |- m : B
-where "Γ |- m : A" := (clc_type Γ m A).
+  Γ ⊢ m : A ->
+  [Γ] ⊢ B : s @ i ->
+  Γ ⊢ m : B
+where "Γ ⊢ m : A" := (clc_type Γ m A).
 
 Inductive ok : context term -> Prop :=
 | nil_ok :
   ok nil
 | ty_ok Γ A s l :
   ok Γ ->
-  [Γ] |- A : s @ l ->
+  [Γ] ⊢ A : s @ l ->
   ok (A :{s} Γ)
 | n_ok Γ :
   ok Γ ->
