coq/cclc/clc_inversion.v
@@ -1,0 +1,24 @@
+From mathcomp Require Import ssreflect ssrbool eqtype ssrnat seq.
+From Coq Require Import ssrfun Utf8 Classical.
+Require Import AutosubstSsr ARS 
+  clc_context clc_ast clc_confluence clc_subtype clc_typing
+  clc_weakening clc_substitution.
+
+Ltac solve_sub :=
+  match goal with
+  | [ H : _ <: _ |- _ ] =>
+    let A := fresh "A" in
+    let B := fresh "B" in
+    let sb := fresh "sb" in
+    let c1 := fresh "c1" in
+    let c2 := fresh "c2" in
+    destruct H as [A B sb c1 c2]; destruct sb
+  end;
+  match goal with
+  | [ c1 : ?A === ?x, c2 : ?x === ?B |- _ ] => 
+    assert (A === B) by 
+      (eapply conv_trans; try solve [apply c1| apply c2]);
+    clear c1 c2;
+    solve_conv
+  | _ => solve_conv
+  end.
